nola/iris/na_inv_deriv.v
@@ -2,7 +2,7 @@
 
 From nola.iris Require Export util deriv na_inv.
 From iris.proofmode Require Import proofmode.
-Import JudgIntpNotation DerivNotation.
+Import PintpNotation DerivNotation.
 
 Section na_inv_deriv.
   Context `{!na_inv'GS PROP Σ, !invGS_gen hlc Σ, !na_invG Σ}.
@@ -15,25 +15,22 @@ Section na_inv_deriv.
 
   (** Derivability data for [na_inv] *)
   Class DerivNaInv (JUDG : judg (iProp Σ)) := DERIV_NA_INV {
-    deriv_na_inv_intp : deriv_ty JUDG (iProp Σ) → PROP $o iProp Σ → iProp Σ;
+    deriv_na_inv_intp ::
+      Pintp (deriv JUDG (iProp Σ)) (PROP $o iProp Σ) (iProp Σ);
     deriv_na_inv_ne {δ} :: NonExpansive (deriv_na_inv_intp δ);
     deriv_na_inv_acsr : na_inv_pool_name → namespace → PROP $o iProp Σ → JUDG;
     deriv_na_inv_acsr_intp {δ p N P} :
-      ⟦ deriv_na_inv_acsr p N P ⟧(δ) ≡
-        na_inv_acsr' (deriv_na_inv_intp δ) p N (deriv_na_inv_intp δ P);
+      ⟦ deriv_na_inv_acsr p N P ⟧(δ) ≡ na_inv_acsr' ⟦⟧(δ) p N (⟦ P ⟧(δ));
   }.
 End na_inv_deriv.
 Notation na_inv_ascr δ p N P := (na_inv_acsr' (deriv_na_inv_intp δ) p N P).
 
 Section na_inv_deriv.
-  Local Notation "⟦ P ⟧' ( δ )" := (deriv_na_inv_intp δ P)
-    (format "'[' ⟦  P  ⟧' '/  ' ( δ ) ']'") : nola_scope.
-  Local Notation "⟦ P ⟧'" := (⟦ P ⟧'(der)).
-
   Context `{!na_inv'GS PROP Σ, !invGS_gen hlc Σ, !na_invG Σ, !DerivNaInv JUDG}.
+  Implicit Type P Q : PROP $o iProp Σ.
 
   (** [na_inv']: Relaxed na_invariant *)
-  Definition na_inv' δ p N P : iProp Σ := □ δ ⸨ deriv_na_inv_acsr p N P ⸩.
+  Definition na_inv' δ p N P : iProp Σ := □ ⸨ deriv_na_inv_acsr p N P ⸩(δ).
 
   (** [na_inv'] is persistent *)
   Fact na_inv'_persistent {δ p N P} : Persistent (na_inv' δ p N P).
@@ -45,8 +42,8 @@ Section na_inv_deriv.
   (** Access [na_inv'] *)
   Lemma na_inv'_acc {p N P E F} : ↑N ⊆ E → ↑N ⊆ F →
     na_own p F -∗ na_inv' der p N P =[na_inv_wsatd der]{E}=∗
-      na_own p (F∖↑N) ∗ ⟦ P ⟧' ∗
-      (na_own p (F∖↑N) -∗ ⟦ P ⟧' =[na_inv_wsatd der]{E}=∗ na_own p F).
+      na_own p (F∖↑N) ∗ ⟦ P ⟧(der) ∗
+      (na_own p (F∖↑N) -∗ ⟦ P ⟧(der) =[na_inv_wsatd der]{E}=∗ na_own p F).
   Proof.
     iIntros (NE NF) "F accP". iDestruct (der_sound with "accP") as "accP".
     rewrite deriv_na_inv_acsr_intp. iApply ("accP" $! _ _ NE NF with "F").
@@ -64,14 +61,14 @@ Section na_inv_deriv.
 
   (** Allocate [na_inv'] *)
   Lemma na_inv'_alloc_rec p P N :
-    (na_inv' δ p N P -∗ ⟦ P ⟧'(δ)) =[na_inv_wsatd δ]=∗ na_inv' δ p N P.
+    (na_inv' δ p N P -∗ ⟦ P ⟧(δ)) =[na_inv_wsatd δ]=∗ na_inv' δ p N P.
   Proof. rewrite -na_inv_tok_na_inv'. exact: na_inv_tok_alloc_rec. Qed.
-  Lemma na_inv'_alloc p P N : ⟦ P ⟧'(δ) =[na_inv_wsatd δ]=∗ na_inv' δ p N P.
+  Lemma na_inv'_alloc p P N : ⟦ P ⟧(δ) =[na_inv_wsatd δ]=∗ na_inv' δ p N P.
   Proof. rewrite -na_inv_tok_na_inv'. exact: na_inv_tok_alloc. Qed.
 
   (** Convert [na_inv'] with [acsr] *)
   Lemma na_inv'_acsr {p N P Q} :
-    □ (∀ δ, acsr (fupd ∅ ∅) ⟦ P ⟧'(δ) ⟦ Q ⟧'(δ)) -∗
+    □ (∀ δ, acsr (fupd ∅ ∅) ⟦ P ⟧(δ) ⟦ Q ⟧(δ)) -∗
     na_inv' δ p N Q -∗ na_inv' δ p N P.
   Proof.
     iIntros "#QPQ #accQ !>". iApply Deriv_byintp. iIntros (? _ _) "#→ _".
@@ -86,14 +83,14 @@ Section na_inv_deriv.
 
   (** Split [na_inv'] over [∗] *)
   Local Lemma na_inv'_sep' {p N PQ P Q} :
-    (∀ δ, ⟦ PQ ⟧'(δ) ≡ (⟦ P ⟧'(δ) ∗ ⟦ Q ⟧'(δ))%I) →
+    (∀ δ, ⟦ PQ ⟧(δ) ≡ (⟦ P ⟧(δ) ∗ ⟦ Q ⟧(δ))%I) →
     na_inv' δ p N PQ ⊢ na_inv' δ p N P.
   Proof.
     iIntros (eq). iApply (na_inv'_acsr with "[]"). iIntros "!>" (?).
     unfold acsr. rewrite eq. iApply (acsr_sep_l (M:=fupd _ _)).
   Qed.
   Lemma na_inv'_sep {p N PQ P Q} :
-    (∀ δ, ⟦ PQ ⟧'(δ) ≡ (⟦ P ⟧'(δ) ∗ ⟦ Q ⟧'(δ))%I) →
+    (∀ δ, ⟦ PQ ⟧(δ) ≡ (⟦ P ⟧(δ) ∗ ⟦ Q ⟧(δ))%I) →
     na_inv' δ p N PQ ⊢ na_inv' δ p N P ∗ na_inv' δ p N Q.
   Proof.
     iIntros (eq) "#i". iSplit; [by iApply na_inv'_sep'|].
@@ -102,7 +99,7 @@ Section na_inv_deriv.
 
   (** Merge [na_inv']s with [∗] *)
   Lemma na_inv'_merge {p N1 N2 N P Q PQ} : N1 ## N2 → ↑N1 ∪ ↑N2 ⊆@{coPset} ↑N →
-    (∀ δ, ⟦ PQ ⟧'(δ) ≡ (⟦ P ⟧'(δ) ∗ ⟦ Q ⟧'(δ))%I) →
+    (∀ δ, ⟦ PQ ⟧(δ) ≡ (⟦ P ⟧(δ) ∗ ⟦ Q ⟧(δ))%I) →
     na_inv' δ p N1 P -∗ na_inv' δ p N2 Q -∗ na_inv' δ p N PQ.
   Proof.
     iIntros (?? eq) "#i #i' !>". iApply (Deriv_map2 with "[] i i'").
