nola/iris/sinv_deriv.v
@@ -2,43 +2,38 @@
 
 From nola.iris Require Export util deriv sinv.
 From iris.proofmode Require Import proofmode.
-Import JudgIntpNotation DerivNotation.
+Import PintpNotation DerivNotation.
+
+(** Derivability data for [sinv] *)
+Class DerivSinv {PROP Σ} (JUDG : judg (iProp Σ)) := DERIV_SINV {
+  deriv_sinv_intp ::
+    Pintp (deriv JUDG (iProp Σ)) (PROP $o iProp Σ) (iProp Σ);
+  deriv_sinv_ne {δ} :: NonExpansive (deriv_sinv_intp δ);
+  deriv_sinv_acsr : PROP $o iProp Σ → PROP $o iProp Σ → JUDG;
+  deriv_sinv_mod : iProp Σ → iProp Σ;
+  deriv_sinv_mod_gen_upd :: GenUpd deriv_sinv_mod;
+  deriv_sinv_acsr_intp {δ P Q} :
+    ⟦ deriv_sinv_acsr P Q ⟧(δ) ≡ acsr deriv_sinv_mod ⟦ P ⟧(δ) ⟦ Q ⟧(δ);
+}.
+(** Notation *)
+Notation sinv_wsatd δ := (sinv_wsat ⟦⟧(δ)).
 
 Section sinv_deriv.
-  Context `{!sinvGS PROP Σ}.
-
-  (** Derivability data for [sinv] *)
-  Class DerivSinv (JUDG : judg (iProp Σ)) := DERIV_SINV {
-    deriv_sinv_intp : deriv_ty JUDG (iProp Σ) → PROP $o iProp Σ → iProp Σ;
-    deriv_sinv_ne {δ} :: NonExpansive (deriv_sinv_intp δ);
-    deriv_sinv_acsr : PROP $o iProp Σ → PROP $o iProp Σ → JUDG;
-    deriv_sinv_mod : iProp Σ → iProp Σ;
-    deriv_sinv_mod_gen_upd :: GenUpd deriv_sinv_mod;
-    deriv_sinv_acsr_intp {δ P Q} :
-      ⟦ deriv_sinv_acsr P Q ⟧(δ) ≡
-        acsr deriv_sinv_mod (deriv_sinv_intp δ P) (deriv_sinv_intp δ Q);
-  }.
-  Local Notation "⟦ P ⟧' ( δ )" := (deriv_sinv_intp δ P)
-    (format "'[' ⟦  P  ⟧' '/  ' ( δ ) ']'") : nola_scope.
-  Local Notation "⟦ P ⟧'" := (⟦ P ⟧'(der)).
-
-  Context `{!DerivSinv JUDG}.
+  Context `{!sinvGS PROP Σ, !DerivSinv (PROP:=PROP) (Σ:=Σ) JUDG}.
+  Implicit Type P Q : PROP $o iProp Σ.
 
   (** [sinv]: Relaxed simple invariant *)
   Definition sinv δ P : iProp Σ :=
-    ∃ Q, □ δ ⸨ deriv_sinv_acsr P Q ⸩ ∗ sinv_tok Q.
+    ∃ Q, □ ⸨ deriv_sinv_acsr P Q ⸩(δ) ∗ sinv_tok Q.
 
   (** [sinv] is persistent *)
   Fact sinv_persistent {δ P} : Persistent (sinv δ P).
   Proof. exact _. Qed.
 
-  (** World satisfaction *)
-  Definition sinv_wsatd δ := sinv_wsat (deriv_sinv_intp δ).
-
   (** Access [sinv] *)
   Lemma sinv_acc {P} :
-    sinv der P -∗ sinv_wsatd der -∗
-      deriv_sinv_mod (⟦ P ⟧' ∗ (⟦ P ⟧' -∗ deriv_sinv_mod (sinv_wsatd der))).
+    sinv der P -∗ sinv_wsatd der -∗ deriv_sinv_mod
+      (⟦ P ⟧(der) ∗ (⟦ P ⟧(der) -∗ deriv_sinv_mod (sinv_wsatd der))).
   Proof.
     iIntros "[%Q[QPQ s]] W". iDestruct (der_sound with "QPQ") as "QPQ".
     rewrite deriv_sinv_acsr_intp.
@@ -57,17 +52,17 @@ Section sinv_deriv.
   Qed.
 
   (** Allocate [sinv] *)
-  Lemma sinv_alloc P : sinv_wsatd δ ==∗ sinv δ P ∗ (⟦ P ⟧'(δ) -∗ sinv_wsatd δ).
+  Lemma sinv_alloc P : sinv_wsatd δ ==∗ sinv δ P ∗ (⟦ P ⟧(δ) -∗ sinv_wsatd δ).
   Proof. rewrite -sinv_tok_sinv. exact: sinv_tok_alloc. Qed.
 
   (** Convert [sinv] with [acsr] *)
-  Lemma sinv_acsr' {P Q} : □ δ ⸨ deriv_sinv_acsr P Q ⸩ -∗ sinv δ Q -∗ sinv δ P.
+  Lemma sinv_acsr' {P Q} : □ ⸨ deriv_sinv_acsr P Q ⸩(δ) -∗ sinv δ Q -∗ sinv δ P.
   Proof.
     iIntros "#QPQ [%R[#RQR $]] !>". iApply (Deriv_map2 with "[] QPQ RQR").
     iIntros (? _ _). rewrite !deriv_sinv_acsr_intp. iApply acsr_trans.
   Qed.
   Lemma sinv_acsr {P Q} :
-    □ (∀ δ, acsr deriv_sinv_mod ⟦ P ⟧'(δ) ⟦ Q ⟧'(δ)) -∗ sinv δ Q -∗ sinv δ P.
+    □ (∀ δ, acsr deriv_sinv_mod ⟦ P ⟧(δ) ⟦ Q ⟧(δ)) -∗ sinv δ Q -∗ sinv δ P.
   Proof.
     iIntros "#PQP". iApply sinv_acsr'. iModIntro. iApply Deriv_intro.
     iIntros (? _ _). rewrite deriv_sinv_acsr_intp. by iApply "PQP".
@@ -75,12 +70,12 @@ Section sinv_deriv.
 
   (** Split [sinv] over [∗] *)
   Local Lemma sinv_sep' {PQ P Q} :
-    (∀ δ, ⟦ PQ ⟧'(δ) ≡ (⟦ P ⟧'(δ) ∗ ⟦ Q ⟧'(δ))%I) → sinv δ PQ ⊢ sinv δ P.
+    (∀ δ, ⟦ PQ ⟧(δ) ≡ (⟦ P ⟧(δ) ∗ ⟦ Q ⟧(δ))%I) → sinv δ PQ ⊢ sinv δ P.
   Proof.
     move=> eq. iApply sinv_acsr. iIntros "!>" (?). unfold acsr. rewrite eq.
     iApply acsr_sep_l.
   Qed.
-  Lemma sinv_sep {PQ P Q} : (∀ δ, ⟦ PQ ⟧'(δ) ≡ (⟦ P ⟧'(δ) ∗ ⟦ Q ⟧'(δ))%I) →
+  Lemma sinv_sep {PQ P Q} : (∀ δ, ⟦ PQ ⟧(δ) ≡ (⟦ P ⟧(δ) ∗ ⟦ Q ⟧(δ))%I) →
     sinv δ PQ ⊢ sinv δ P ∗ sinv δ Q.
   Proof.
     iIntros (eq) "#s". iSplit; [by iApply sinv_sep'|].
