nola/util/intp.v
@@ -1,0 +1,14 @@
+(** * Interpretation *)
+
+From nola Require Export prelude.
+
+(** Parameterized interpretation *)
+Class Pintp (X A B : Type) := pintp : X → A → B.
+Hint Mode Pintp - ! - : typeclass_instances.
+Module PintpNotation.
+  Notation "⟦ ⟧( x )" := (pintp x) (format "⟦ ⟧( x )") : nola_scope.
+  Notation "⟦ ⟧( x )@{ A }" := (pintp (A:=A) x) (only parsing) : nola_scope.
+  Notation "⟦ a ⟧( x )" := (pintp x a) (format "⟦  '[' a  ']' ⟧( x )")
+    : nola_scope.
+  Notation "⟦ a ⟧( x )@{ A }" := (pintp (A:=A) x a) (only parsing) : nola_scope.
+End PintpNotation.
