README.md
@@ -64,6 +64,7 @@ All the Coq code is in [`nola/`](nola/) and structured as follows:
   + [`prod`](nola/util/prod.v) (Modified product),
     [`plist`](nola/util/plist.v) (Product list)
   + [`proph`](nola/util/proph.v) (Prophecy)
+  + [`intp`](nola/util/intp.v) (Interpretation)
 - [`iris/`](nola/iris) : Iris libraries
   + [`ofe`](nola/iris/ofe.v) (OFEs)
   + [`list`](nola/iris/list.v) (On `list`),
